wip

src/drf/AbortProp.v
@@ -31,6 +31,7 @@ Require Import Program.
 Require Import Cell.
 Require Import Time.
 Require Import PredStep.
+Require Import ReorderPromises2.
 
 Require Import DRF_PF.
 
@@ -61,11 +62,9 @@ Proof.
   econs. ss. eapply Time.bot_spec.
 Qed.
 
-Definition is_cancel (e: ThreadEvent.t) : Prop :=
-  match e with
-  | ThreadEvent.promise _ _ _ _ Memory.op_kind_cancel => True
-  | _ => False
-  end.
+Definition no_reserves (proms: Memory.t): Prop :=
+  forall loc to from msg (GET: Memory.get loc to proms = Some (from, msg)),
+    msg <> Message.reserve.
 
 Inductive only_reserves (proms: Memory.t): Prop :=
 | only_reserves_intro
@@ -118,66 +117,6 @@ Proof.
       i. exploit FINITE; eauto. i. des; clarify.
 Qed.
 
-Inductive concreter_memory (mem_src mem_tgt: Memory.t): Prop :=
-| concreter_memory_intro
-    (COVER: forall loc to (COV: covered loc to mem_src),
-        covered loc to mem_tgt)
-    (MSG: forall loc to from vw val
-                 (GETTGT: Memory.get loc to mem_tgt = Some (from, Message.full val vw)),
-        Memory.get loc to mem_src = Some (from, Message.full val vw))
-.
-
-(* Lemma concreter_memory_write mem_src0 mem_tgt0 prom0 *)
-(*       loc from to val vw_src vw_tgt prom1 mem_tgt1 kind *)
-(*       (CONCRETE: concreter_memory mem_src0 mem_tgt0) *)
-(*       (MLESRC: Memory.le prom0 mem_src0) *)
-(*       (MLETGT: Memory.le prom0 mem_tgt0) *)
-(*       (VWLE: View.opt_le vw_src vw_tgt) *)
-(*       (VWWF: View.opt_wf vw_src) *)
-(*       (WRITE: Memory.write prom0 mem_tgt0 loc from to val vw_tgt prom1 mem_tgt1 kind) *)
-(*   : *)
-(*     exists mem_src1, *)
-(*       (<<PROMISE: Memory.write prom0 mem_src0 loc from to val vw_src prom1 mem_src1 kind>>) /\ *)
-(*       (<<CONCRETE: concreter_memory mem_src1 mem_tgt1>>). *)
-(* Proof. *)
-(*   inv WRITE. inv PROMISE. *)
-(*   - exploit add_succeed_wf; try apply PROMISES. i. des. *)
-(*     exploit add_succeed_wf; try apply MEM. i. des. *)
-
-Lemma concreter_memory_step
-      lang prom th_src th_tgt th_tgt' st st' vw vw' prom' sc sc'
-      mem_src mem_tgt mem_tgt' tf e
-      (VWF: TView.wf vw)
-      (TH_SRC: th_src = Thread.mk lang st (Local.mk vw prom) sc mem_src)
-      (TH_TGT0: th_tgt = Thread.mk lang st (Local.mk vw prom) sc mem_tgt)
-      (TH_TGT1: th_tgt' = Thread.mk lang st' (Local.mk vw' prom') sc' mem_tgt')
-      (CONCRETE: concreter_memory mem_src mem_tgt)
-      (MLESRC: Memory.le prom mem_src)
-      (MLETGT: Memory.le prom mem_tgt)
-      (STEP: Thread.step tf e th_tgt th_tgt')
-  :
-    exists v_src' mem_src' sc_src',
-      (<<STEP: Thread.step
-                 tf e th_src
-                 (Thread.mk lang st' (Local.mk v_src' prom') sc_src' mem_src')>>) /\
-      (<<CONCRETE: concreter_memory mem_src' mem_tgt'>>)
-.
-Proof.
-Admitted.
-
-Lemma progressable_in_added_rtc
-      lang st lc sc0 sc1 m0 m1 tm
-      (CONSISTENT: Thread.consistent (Thread.mk lang st lc sc0 m0))
-      (FUTURE: Memory.future m0 m1)
-  :
-    exists m2 e2,
-      (<<ADDED: rtc (added_memory tm) m1 m2>>) /\
-      (<<STEPS: rtc (Thread.tau_step (lang:=lang))
-                    (Thread.mk _ st lc sc1 m1) e2>>) /\
-      (<<PROMISES: Local.promises (Thread.local e2) = Memory.bot>>).
-Proof.
-Admitted.
-
 Lemma promise_free_no_promise P lang (th0 th1: Thread.t lang) e
       (NOPROMISE: th0.(Thread.local).(Local.promises) = Memory.bot)
       (STEP: pred_step (P /1\ promise_free) e th0 th1)
@@ -220,25 +159,320 @@ Proof.
       * econs; eauto. econs; eauto.
 Qed.
 
+Definition caps (mem0 prom : Memory.t) (l : Loc.t) (t from : Time.t) (msg : Message.t) :=
+  forall mem1 (CAP: Memory.cap prom mem0 mem1),
+    (<<GET0: Memory.get l t mem0 = None>>) /\
+    (<<GET1: Memory.get l t mem1 = Some (from, msg)>>).
+
+(* Inductive my_caps (mem0 prom : Memory.t) (l : Loc.t) (t from : Time.t) (msg : Message.t) := *)
+(*   (<<CAPS: caps mem0 prom l t from msg>>) /\ *)
+(*   (<< *)
+
+
+
+(*   forall mem1 (CAP: Memory.cap prom mem0 mem1), *)
+(*     (<<GET0: Memory.get l t mem0 = None>>) /\ *)
+(*     (<<GET1: Memory.get l t mem1 = Some (from, msg)>>). *)
+
+
+Definition caps_loc (mem0 prom : Memory.t) (l : Loc.t) (t : Time.t): Prop :=
+  exists from msg, (<<CAPS: caps mem0 prom l t from msg>>).
+
+Lemma caps_unchangable mem0 prom mem1
+      (MLE: Memory.le prom mem0)
+      (CAP: Memory.cap prom mem0 mem1)
+  :
+    caps mem0 prom <4= unchangable mem1 prom.
+Proof.
+  i. exploit PR; eauto. i. des. inv CAP.
+  econs; eauto. ii. inv H.
+  destruct msg. eapply MLE in GET. clarify.
+Qed.
+
+Lemma finite_least P (l: list Time.t)
+  :
+    (exists to,
+        (<<SAT: P to>>) /\
+        (<<IN: List.In to l>>) /\
+        (<<LEAST: forall to'
+                         (IN: List.In to' l)
+                         (SAT: P to'),
+            Time.le to to'>>)) \/
+    (<<EMPTY: forall to (IN: List.In to l), ~ P to>>).
+Proof.
+  induction l.
+  - right. ii. inv IN.
+  - destruct (classic (P a)).
+    + des.
+      * destruct (Time.le_lt_dec a to).
+        { left. exists a. esplits; ss; eauto.
+          i. des; clarify; eauto. refl. }
+        { left. exists to. esplits; ss; eauto.
+          i. des; clarify; eauto. left. eauto. }
+      * left. exists a. esplits; ss; eauto.
+        i. des; clarify.
+        { refl. }
+        { exfalso. eapply EMPTY; eauto. }
+    + des.
+      * left. esplits; ss; eauto.
+        i. des; clarify. eapply LEAST; eauto.
+      * right. ii. ss. des; clarify.
+        eapply EMPTY; eauto.
+Qed.
+
+Lemma cell_elements_least cell P
+  :
+    (exists to from msg,
+        (<<GET: Cell.get to cell = Some (from, msg)>>) /\
+        (<<SAT: P to>>) /\
+        (<<LEAST: forall to' from' msg'
+                         (GET': Cell.get to' cell = Some (from', msg'))
+                         (SAT: P to'),
+            Time.le to to'>>)) \/
+    (<<EMPTY: forall to from msg
+                     (GET: Cell.get to cell = Some (from, msg)),
+        ~ P to>>).
+Proof.
+  hexploit (Cell.finite cell). i. des.
+  hexploit (finite_least (fun to => P to /\ exists from msg, Cell.get to cell = Some (from, msg)) dom).
+  i. des.
+  - left. esplits; eauto. i.
+    dup GET'. eapply H in GET'. eauto.
+  - right. ii. dup GET. eapply H in GET0.
+    eapply EMPTY in GET0. eapply GET0.
+    esplits; eauto.
+Qed.
+
+Lemma disjoint_equivalent2 from0 to0 from1 to1
+  :
+    (<<DISJOINT: Interval.disjoint (from0, to0) (from1, to1)>>) <->
+    ((<<TS0: ~ Time.lt from0 to0>>) \/ (<<TS1: ~ Time.lt from1 to1>>) \/
+     (<<TS0: Time.le (Time.meet to0 to1) (Time.join from0 from1)>>)).
+Proof.
+  set (disjoint_equivalent from0 to0 from1 to1).
+  eapply not_iff_compat in i. split; i.
+  - des. hexploit i.
+    { ii. clarify. } i.
+    apply not_and_or in H0. des; eauto.
+    apply not_and_or in H0. des; eauto.
+    right. right. red.
+    destruct (Time.le_lt_dec (Time.meet to0 to1) (Time.join from0 from1)); eauto.
+    exfalso. eauto.
+  - destruct i. hexploit H1.
+    { ii. des; eauto. eapply Time.lt_strorder.
+      eapply TimeFacts.lt_le_lt; eauto. }
+    ii. eauto.
+Qed.
+
+Lemma or_strengthen A B
+      (OR: A \/ B)
+  :
+    (A \/ ((<<NOT: ~ A>>) /\ (<<SAT: B>>))).
+Proof.
+  destruct (classic A); eauto. des; eauto.
+Qed.
+
+Lemma memory_get_ts_strong loc to mem from msg
+      (GET: Memory.get loc to mem = Some (from, msg))
+  :
+    (from = Time.bot /\ to = Time.bot) \/
+    ((<<TS: Time.lt from to>>) /\ (<<TO: to <> Time.bot>>)).
+Proof.
+  apply Memory.get_ts in GET.
+  destruct (classic (to = Time.bot)); clarify.
+  - des; clarify; eauto.
+    exfalso. eapply Time.lt_strorder.
+    eapply TimeFacts.lt_le_lt; eauto. eapply Time.bot_spec.
+  - des; clarify. right. eauto.
+Qed.
+
+Lemma memory_get_from_inj mem loc from to0 to1 msg0 msg1
+      (GET0: Memory.get loc to0 mem = Some (from, msg0))
+      (GET1: Memory.get loc to1 mem = Some (from, msg1))
+  :
+    (<<TO: to0 = to1>>) \/
+    (((<<BOT: to0 = Time.bot>>) \/ (<<BOT: to1 = Time.bot>>)) /\ (<<BOT: from = Time.bot>>) /\
+     (<<TO: to0 <> to1>>)).
+Proof.
+  exploit Memory.get_disjoint.
+  - eapply GET0.
+  - eapply GET1.
+  - i. des; clarify; eauto.
+    eapply memory_get_ts_strong in GET0.
+    eapply memory_get_ts_strong in GET1.
+    des; clarify; eauto.
+    { right. esplits; eauto. }
+    { right. esplits; eauto. }
+    exfalso. eapply x0.
+    + instantiate (1:=Time.meet to0 to1). econs; ss; eauto.
+      * unfold Time.meet. des_ifs.
+      * eapply Time.meet_l.
+    + econs; ss; eauto.
+      * unfold Time.meet. des_ifs.
+      * eapply Time.meet_r.
+Qed.
+
+
+Lemma memory_get_to_mon mem loc from0 from1 to0 to1 msg0 msg1
+      (GET0: Memory.get loc to0 mem = Some (from0, msg0))
+      (GET1: Memory.get loc to1 mem = Some (from1, msg1))
+      (TO: Time.lt from0 from1)
+  :
+    Time.lt to0 to1.
+Proof.
+  exploit Memory.get_disjoint.
+  - eapply GET0.
+  - eapply GET1.
+  - i. des; clarify.
+    + exfalso. eapply Time.lt_strorder. eauto.
+    + dup GET0. dup GET1.
+      eapply memory_get_ts_strong in GET0.
+      eapply memory_get_ts_strong in GET1.
+      des; clarify.
+      * exfalso. eapply Time.lt_strorder.
+        eapply TimeFacts.lt_le_lt; eauto. eapply Time.bot_spec.
+      * hexploit (Time.bot_spec from1). i.
+        destruct H; eauto.
+      * eapply disjoint_equivalent2 in x0. des; clarify.
+        unfold Time.meet, Time.join in *. des_ifs; eauto.
+        { destruct l; eauto. destruct H; eauto. clarify.
+          exfalso. eapply Time.lt_strorder; eauto. }
+        { destruct l; eauto. destruct H; eauto. clarify.
+          exfalso. eapply Time.lt_strorder; eauto. }
+        { exfalso. eapply Time.lt_strorder.
+          eapply TimeFacts.le_lt_lt; eauto. }
+        { exfalso. eapply Time.lt_strorder.
+          eapply TimeFacts.le_lt_lt; eauto. }
+Qed.
+
+Lemma memory_get_from_mon mem loc from0 from1 to0 to1 msg0 msg1
+      (GET0: Memory.get loc to0 mem = Some (from0, msg0))
+      (GET1: Memory.get loc to1 mem = Some (from1, msg1))
+      (TO: Time.lt to0 to1)
+  :
+    (<<FROMTO: Time.le to0 from1>>) \/
+    ((<<FROM0: from0 = Time.bot>>) /\ (<<FROM1: from1 = Time.bot>>) /\ (<<TO: to0 = Time.bot>>)).
+Proof.
+  exploit Memory.get_disjoint.
+  - eapply GET0.
+  - eapply GET1.
+  - i. des; clarify.
+    + exfalso. eapply Time.lt_strorder. eauto.
+    + dup GET0. dup GET1.
+      eapply memory_get_ts_strong in GET0.
+      eapply memory_get_ts_strong in GET1.
+      des; clarify.
+      * exfalso. eapply Time.lt_strorder.
+        eapply TimeFacts.lt_le_lt; eauto. eapply Time.bot_spec.
+      * exfalso. eapply Time.lt_strorder.
+        eapply TimeFacts.lt_le_lt; eauto. eapply Time.bot_spec.
+      * left. apply Time.bot_spec.
+      * left. destruct (Time.le_lt_dec to0 from1); auto. exfalso.
+        eapply x0.
+        { instantiate (1:=to0).
+          econs; ss. refl. }
+        { econs; ss. left. auto. }
+Qed.
+
+(* Lemma memory_get_from_mon2 mem loc from0 from1 to0 to1 msg0 msg1 *)
+(*       (GET0: Memory.get loc to0 mem = Some (from0, msg0)) *)
+(*       (GET1: Memory.get loc to1 mem = Some (from1, msg1)) *)
+(*       (TO: Time.lt to0 to1) *)
+(*   : *)
+(*     (<<FROM: Time.lt from0 from1>>) \/ *)
+(*     ((<<FROM0: from0 = Time.bot>>) /\ (<<FROM1: from1 = Time.bot>>) /\ (<<TO: to0 = Time.bot>>)). *)
+(* Proof. *)
+(* Admitted. *)
+
+Lemma caps_concrete_last mem0 prom mem1 tm l t from val released
+      (RESERVE: Memory.reserve_wf prom mem0)
+      (INHABITED: Memory.inhabited mem0)
+      (MAX: Memory.max_full_timemap mem0 tm)
+      (CAP: Memory.cap prom mem0 mem1)
+      (CAPS: caps mem0 prom l t from (Message.full val released))
+  :
+    from = Memory.max_ts l mem0.
+Proof.
+  exploit CAPS; eauto. i. des. inv CAP.
+  exploit COMPLETE; eauto. i. des.
+  destruct (classic (Memory.max_ts l mem0 = from)); eauto. exfalso.
+  set (@cell_elements_least
+         (mem0 l)
+         (fun to => Time.lt from to)). des.
+  + assert (TLE: Time.le from from0).
+    { dup GET. eapply Memory.get_ts in GET. des; clarify.
+      { exfalso. eapply Time.lt_strorder.
+        eapply TimeFacts.lt_le_lt; eauto. eapply Time.bot_spec. }
+      exploit memory_get_from_mon.
+      - eapply x.
+      - eapply GET2.
+      - eauto.
+      - i. des; clarify. refl. }
+    destruct TLE.
+    * exploit MIDDLE; eauto.
+      econs.
+      { eapply x. }
+      { eapply GET. }
+      { eauto. }
+      { i. destruct (Memory.get l ts mem0) eqn: GET2; auto.
+        destruct p. exfalso. dup GET2. eapply LEAST in GET2; eauto.
+        eapply Memory.get_ts in GET. des; clarify.
+        - eapply Time.lt_strorder. eapply TimeFacts.lt_le_lt.
+          eapply SAT. eapply Time.bot_spec.
+        - eapply Time.lt_strorder. eapply TimeFacts.lt_le_lt.
+          eapply GET. etrans; eauto. }
+      { i. exploit memory_get_from_inj.
+        - eapply x1.
+        - eapply GET1.
+        - i. des; clarify. eapply Time.lt_strorder; eauto. }
+    * destruct H0.
+      exploit memory_get_from_inj.
+      { eapply GET1. }
+      { eapply SOUND. eapply GET. }
+      { i. des; clarify.
+        - unfold Memory.get in GET0. clarify.
+        - eapply Time.lt_strorder; eauto. }
+  + exploit Memory.max_ts_spec.
+    { eapply x. } i. des.
+    eapply EMPTY; eauto. destruct MAX0; clarify.
+    exfalso. eauto.
+Qed.
+
+Lemma caps_max_view mem0 prom mem1 tm l t from val released
+      (RESERVE: Memory.reserve_wf prom mem0)
+      (INHABITED: Memory.inhabited mem0)
+      (MAX: Memory.max_full_timemap mem0 tm)
+      (CAP: Memory.cap prom mem0 mem1)
+      (CAPS: caps mem0 prom l t from (Message.full val released))
+  :
+    (<<FROM: from = Memory.max_ts l mem0>>) /\
+    (<<RESERVE: Memory.latest_reserve l prom mem0>>) /\
+    (<<VAL: Memory.latest_val l mem0 val >>) /\
+    (<<RELEASED: released = Some (View.mk tm tm)>>) /\
+    (<<TO: t = Time.incr (Memory.max_ts l mem0)>>).
+Proof.
+  exploit caps_concrete_last; eauto. i. clarify.
+  exploit CAPS; eauto. i. des. inv CAP.
+  exploit COMPLETE; eauto. i. des.
+  exploit Memory.latest_val_exists; eauto. i. des.
+  exploit BACK; eauto. i.
+  exploit memory_get_from_inj.
+  { eapply x1. }
+  { eapply GET1. } i. des; clarify.
+  - esplits; eauto.
+  - exfalso. eapply Time.lt_strorder. eapply TimeFacts.lt_le_lt.
+    + eapply Time.incr_spec.
+    + erewrite BOT0. eapply Time.bot_spec.
+  - erewrite INHABITED in GET0. clarify.
+Qed.
+
 Definition pf_consistent_strong lang (e:Thread.t lang): Prop :=
   forall mem1 sc1
          (CAP: Memory.cap e.(Thread.local).(Local.promises) e.(Thread.memory) mem1),
   exists e2,
-    (<<STEPS: rtc (tau (@pred_step (promise_free /1\ no_sc) lang)) (Thread.mk _ e.(Thread.state) e.(Thread.local) sc1 mem1) e2>>) /\
+    (<<STEPS: rtc (tau (@pred_step ((promise_free /1\ no_acq_read_msgs (caps_loc e.(Thread.memory) e.(Thread.local).(Local.promises))) /1\ no_sc) lang)) (Thread.mk _ e.(Thread.state) e.(Thread.local) sc1 mem1) e2>>) /\
     ((<<FAILURE: Local.failure_step e2.(Thread.local)>>) \/
      (<<PROMISES: e2.(Thread.local).(Local.promises) = Memory.bot>>)).
-
-(* Definition pf_consistent_strong lang (e:Thread.t lang): Prop := *)
-(*   forall mem1 sc1 *)
-(*          (WF: Local.wf e.(Thread.local) e.(Thread.memory)) *)
-(*          (MEM: Memory.closed e.(Thread.memory)) *)
-(*          (CAP: Memory.cap e.(Thread.local).(Local.promises) e.(Thread.memory) mem1), *)
-(*   exists e2 e3, *)
-(*     (<<STEPS: rtc (tau (@pred_step (no_sc /1\ promise_free) lang)) (Thread.mk _ e.(Thread.state) e.(Thread.local) sc1 mem1) e2>>) /\ *)
-(*     (<<FAILURE: pred_step (no_sc /1\ promise_free) (ThreadEvent.failure) e2 e3>>) \/ *)
-(*     exists e2, *)
-(*       (<<STEPS: rtc (tau (@pred_step (no_sc /1\ promise_free) lang)) (Thread.mk _ e.(Thread.state) e.(Thread.local) sc1 mem1) e2>>) /\ *)
-(*       (<<PROMISES: e2.(Thread.local).(Local.promises) = Memory.bot>>). *)
 
 Lemma write_promises_decrease prom0 mem0 loc from to val realeased prom1 mem1 kind
       (WRITE: Memory.write prom0 mem0 loc from to val realeased prom1 mem1 kind)
@@ -364,6 +598,17 @@ Proof.
   specialize (MAX loc). inv MAX. eapply MAX0; eauto.
 Qed.
 
+Lemma unchangable_rtc_increase P lang (th0 th1: Thread.t lang)
+      (STEPS: rtc (tau (@pred_step P lang))th0 th1)
+  :
+    unchangable th0.(Thread.memory) th0.(Thread.local).(Local.promises) <4=
+    unchangable th1.(Thread.memory) th1.(Thread.local).(Local.promises).
+Proof.
+  ginduction STEPS; ss. i.
+  eapply IHSTEPS.
+  inv H. inv TSTEP. inv STEP. eapply unchangable_increase; eauto.
+Qed.
+
 Lemma pf_consistent_pf_consistent_strong lang (th: Thread.t lang)
       (WF: Local.wf th.(Thread.local) th.(Thread.memory))
       (MEM: Memory.closed th.(Thread.memory))
@@ -372,67 +617,93 @@ Lemma pf_consistent_pf_consistent_strong lang (th: Thread.t lang)
   :
     pf_consistent_strong th.
 Proof.
+  ii. exploit Memory.max_full_timemap_exists; eauto. intros MAX. des.
   ii. exploit Memory.max_full_timemap_exists.
   { eapply le_inhabited; eauto. eapply Memory.cap_le; eauto. refl. }
   i. des. exploit CONSISTENT; eauto. i.
   destruct x as [e2 [STEPS GOOD]]. guardH GOOD. des.
+  eapply pf_step_promise_free_step_rtc in STEPS.
+  eapply hold_or_not with (Q := no_acq_read_msgs (caps_loc (Thread.memory th) (Local.promises (Thread.local th))) /1\ no_sc) in STEPS. des.
 
-  - eapply pf_step_promise_free_step_rtc in STEPS.
-    eapply hold_or_not with (Q := no_sc) in STEPS. des.
-    + destruct th. destruct e2. ss.
-      exploit no_sc_any_sc_rtc; eauto. i. des.
-      esplits; eauto. unguard. des.
-      * left. ss. inv FAILURE; inv STEP0. inv LOCAL. eauto.
-      * right. esplits; eauto.
+  - destruct th. destruct e2. ss.
+    eapply pred_step_rtc_mon with (Q:=(promise_free /1\ no_acq_read_msgs (caps_loc memory (Local.promises local))) /1\ no_sc) in HOLD; cycle 1.
+    { i. des. esplits; eauto. }
+    exploit no_sc_any_sc_rtc; try eapply HOLD; eauto. i. des.
+    esplits; eauto. unguard. des.
+    + left. ss. inv FAILURE; inv STEP0. inv LOCAL. eauto.
+    + right. esplits; eauto.
 
-    + exploit Thread.rtc_tau_step_future.
-      { eapply thread_steps_pred_steps. eapply STEPS0. }
-      { ss. eapply Local.cap_wf; eauto. }
-      { ss. eapply Memory.max_full_timemap_closed; eauto. }
-      { ss. eapply Memory.cap_closed; eauto. }
-      i. des. ss. inv STEP.
-      exploit Thread.step_future; eauto.
-      i. des.
+  - exploit Thread.rtc_tau_step_future.
+    { eapply thread_steps_pred_steps. eapply STEPS0. }
+    { ss. eapply Local.cap_wf; eauto. }
+    { ss. eapply Memory.max_full_timemap_closed; eauto. }
+    { ss. eapply Memory.cap_closed; eauto. }
+    i. des. ss. inv STEP.
+    exploit Thread.step_future; eauto.
+    i. des.
 
-      hexploit (@rtc_tau_step_promise_consistent _ e3 e2); eauto.
-      { eapply thread_steps_pred_steps; eauto. }
-      { unguard. des.
-        - inv FAILURE; inv STEP. inv LOCAL. inv LOCAL0. ss.
-        - ii. rewrite PROMISES in *.
-          erewrite Memory.bot_get in PROMISE. clarify. } intros PROMS.
+    hexploit (@rtc_tau_step_promise_consistent _ e3 e2); eauto.
+    { eapply thread_steps_pred_steps; eauto. }
+    { unguard. des.
+      - inv FAILURE; inv STEP. inv LOCAL. inv LOCAL0. ss.
+      - ii. rewrite PROMISES in *.
+        erewrite Memory.bot_get in PROMISE. clarify. } intros PROMS.
 
-      assert (RESERVES: only_reserves e2'.(Thread.local).(Local.promises)).
-      { replace (Local.promises (Thread.local e2')) with
-            (Local.promises (Thread.local e3)); cycle 1.
-        { unfold no_sc in BREAKQ. des_ifs.
-          - inv STEP0; inv STEP; ss. inv LOCAL. inv LOCAL0. ss.
-          - inv STEP0; inv STEP; ss. inv LOCAL. inv LOCAL0. ss. }
+    assert (RESERVES: only_reserves e2'.(Thread.local).(Local.promises)).
+    { econs.
+      - i. destruct msg; auto. exfalso. dup STEPS0.
+        eapply pf_step_rtc_promises_decrease in STEPS0; cycle 1.
+        { econs; eauto. }
+        ss. inv STEPS0.
+        unfold no_sc, no_acq_read_msgs in BREAKQ. des_ifs; try by (exfalso; eauto).
+        + apply not_and_or in BREAKQ. des; clarify.
+          apply imply_to_and in BREAKQ. des. apply NNPP in BREAKQ0.
+          unfold caps_loc in *. des. dup CAPS.
+          eapply caps_unchangable in CAPS; eauto; cycle 1.
+          { inv WF. eauto. }
+          eapply unchangable_rtc_increase in STEPS2; eauto. inv STEPS2.
+          inv STEP0; inv STEP. ss. inv LOCAL.
+          inv LOCAL0. clarify. eapply caps_max_view in CAPS0; eauto; cycle 1.
+          { inv WF. eauto. } des.
+          clarify. eapply PROMS in GET. ss. des_ifs. ss.
+          exploit max_full_timemap_get.
+          * apply MAX.
+          * inv WF. eapply PROMISES. eauto.
+          * i. eapply Time.lt_strorder. eapply TimeFacts.lt_le_lt; eauto.
+            etrans; eauto. eapply TimeMap.join_r.
+        + apply not_and_or in BREAKQ. des; clarify.
+          apply imply_to_and in BREAKQ. des. apply NNPP in BREAKQ0.
+          unfold caps_loc in *. des. dup CAPS.
+          eapply caps_unchangable in CAPS; eauto; cycle 1.
+          { inv WF. eauto. }
+          eapply unchangable_rtc_increase in STEPS2; eauto. inv STEPS2.
+          inv STEP0; inv STEP. ss. inv LOCAL.
+          eapply write_step_promise_consistent in LOCAL2; eauto.
+          inv LOCAL1. clarify. eapply caps_max_view in CAPS0; eauto; cycle 1.
+          { inv WF. eauto. } des.
+          clarify. eapply LOCAL2 in GET. ss. des_ifs. ss.
+          exploit max_full_timemap_get.
+          * apply MAX.
+          * inv WF. eapply PROMISES. eauto.
+          * i. eapply Time.lt_strorder. eapply TimeFacts.lt_le_lt; eauto.
+            etrans; eauto. eapply TimeMap.join_r.
+        + apply not_and_or in BREAKQ. des; clarify. apply NNPP in BREAKQ.
+          inv STEP0; inv STEP. ss. inv LOCAL. inv LOCAL0. ss.
+          eapply PROMS in GET. ss. des_ifs. ss.
+          hexploit max_full_timemap_get; eauto.
+          * inv WF. eapply Memory.cap_le; eauto.
+          * i. eapply Time.lt_strorder. eapply TimeFacts.lt_le_lt; eauto.
+        + inv STEP0; inv STEP. ss. inv LOCAL. inv LOCAL0. ss.
+          eapply PROMS in GET. ss. des_ifs. ss.
+          hexploit max_full_timemap_get; eauto.
+          * inv WF. eapply Memory.cap_le; eauto.
+          * i. eapply Time.lt_strorder. eapply TimeFacts.lt_le_lt; eauto.
+      - inv WF2. eauto. }
 
-        assert (MAXVIEW: TimeMap.le
-                           tm
-                           (View.rlx (TView.cur (Local.tview (Thread.local e3))))).
-        { unfold no_sc in BREAKQ. des_ifs.
-          - apply NNPP in BREAKQ. etrans; eauto.
-            inv STEP0; inv STEP; ss. inv LOCAL. inv LOCAL0. ss. des_ifs.
-          - etrans; eauto.
-            inv STEP0; inv STEP; ss. inv LOCAL. inv LOCAL0. ss. }
-
-        econs.
-        - ii. destruct msg; auto. exfalso.
-          eapply pf_step_rtc_promises_decrease in STEPS0; cycle 1.
-          + eapply pf_step_promises_decrease; eauto.
-            * econs; eauto. econs; eauto.
-            * econs; eauto.
-          + ss. inv STEPS0.
-            eapply PROMS in GET.
-            hexploit max_full_timemap_get.
-            * eauto.
-            * inv WF. eapply Memory.cap_le; eauto.
-            * i. eapply Time.lt_strorder. eapply TimeFacts.lt_le_lt; eauto.
-        - inv WF0. eauto. }
-
-      destruct e2'. destruct local. ss.
-      eapply no_sc_any_sc_rtc in STEPS0; ss. des.
+    destruct e2'. destruct local. ss.
+    eapply pred_step_rtc_mon with (Q:=(promise_free /1\ no_acq_read_msgs (caps_loc (Thread.memory th) (Local.promises (Thread.local th)))) /1\ no_sc) in STEPS0; cycle 1.
+    { i. des. esplits; eauto. }
+    eapply no_sc_any_sc_rtc in STEPS0; ss. des.
       exploit reserves_cancelable; eauto.
       { inv WF2. eauto. }
       i. des. esplits.
@@ -442,3 +713,262 @@ Proof.
           unfold is_cancel. i. des_ifs. }
       * ss. eauto.
 Qed.
+
+Lemma promise_not_cacncel_reserves_same prom0 mem0 loc from to msg prom1 mem1 kind
+      (PROM: Memory.promise prom0 mem0 loc from to msg prom1 mem1 kind)
+      (NOTCANCEL: kind <> Memory.op_kind_cancel)
+      loc0 to0 from0
+      (GET: Memory.get loc0 to0 mem0 = Some (from0, Message.reserve))
+  :
+    exists from1,
+      Memory.get loc0 to0 mem1 = Some (from1, Message.reserve).
+Proof.
+  inv PROM.
+  - eapply Memory.add_get1 in GET; eauto.
+  - des. clarify. erewrite Memory.split_o; eauto.
+    dup MEM. eapply Memory.split_get0 in MEM0.
+    eapply split_succeed_wf in MEM. des. des_ifs.
+    + ss. des. clarify.
+    + ss. guardH o. des. clarify.
+      esplits; eauto.
+    + esplits; eauto.
+  - des. clarify. erewrite Memory.lower_o; eauto. des_ifs.
+    + ss. des. clarify.
+      eapply lower_succeed_wf in MEM. des. clarify.
+    + esplits; eauto.
+  - clarify.
+Qed.
+
+Lemma step_not_cancel_reserves_same lang e th0 th1
+      (STEPS: (@pred_step (promise_free /1\ (fun e => ~ is_cancel e)) lang) e th0 th1)
+      loc to from
+      (GET: Memory.get loc to th0.(Thread.memory) = Some (from, Message.reserve))
+  :
+    exists from',
+      Memory.get loc to th1.(Thread.memory) = Some (from', Message.reserve).
+Proof.
+  inv STEPS. inv STEP. inv STEP0.
+  - inv STEP. des. ss. inv LOCAL.
+    eapply promise_not_cacncel_reserves_same; eauto.
+    ii. clarify.
+  - inv STEP. inv LOCAL; ss.
+    + esplits; eauto.
+    + esplits; eauto.
+    + inv LOCAL0. inv WRITE.
+      eapply promise_not_cacncel_reserves_same; eauto.
+      ii. clarify. inv PROMISE. clarify.
+    + inv LOCAL2. inv WRITE.
+      eapply promise_not_cacncel_reserves_same; eauto.
+      ii. clarify. inv PROMISE. clarify.
+    + esplits; eauto.
+    + esplits; eauto.
+    + esplits; eauto.
+Qed.
+
+Lemma steps_not_cancel_reserves_same lang th0 th1
+      (STEPS: rtc (tau (@pred_step (promise_free /1\ (fun e => ~ is_cancel e)) lang)) th0 th1)
+      loc to from
+      (GET: Memory.get loc to th0.(Thread.memory) = Some (from, Message.reserve))
+  :
+    exists from',
+      Memory.get loc to th1.(Thread.memory) = Some (from', Message.reserve).
+Proof.
+  ginduction STEPS; i.
+  - esplits; eauto.
+  - inv H. exploit step_not_cancel_reserves_same; eauto. i. des.
+    exploit IHSTEPS; eauto.
+Qed.
+
+Definition pf_consistent_strong2 lang (e0:Thread.t lang): Prop :=
+  forall mem1 sc1
+         (CAP: Memory.cap e0.(Thread.local).(Local.promises) e0.(Thread.memory) mem1),
+  exists e1 e2,
+    (<<STEPS0: rtc (tau (@pred_step is_cancel lang)) e0 e1>>) /\
+    (<<NORESERVE: no_reserves e1.(Thread.memory)>>) /\
+    (<<STEPS1: rtc (tau (@pred_step ((promise_free /1\ (fun e => ~ is_cancel e) /1\ no_acq_read_msgs (caps_loc e0.(Thread.memory) e0.(Thread.local).(Local.promises))) /1\ no_sc) lang)) (Thread.mk _ e0.(Thread.state) e0.(Thread.local) sc1 mem1) e2>>) /\
+    ((<<FAILURE: Local.failure_step e2.(Thread.local)>>) \/
+     (<<PROMISES: e2.(Thread.local).(Local.promises) = Memory.bot>>)).
+
+
+Lemma pf_consistent_pf_consistent_strong2 lang (th: Thread.t lang)
+      (WF: Local.wf th.(Thread.local) th.(Thread.memory))
+      (MEM: Memory.closed th.(Thread.memory))
+      (INHABITED: Memory.inhabited th.(Thread.memory))
+      (CONSISTENT: pf_consistent th)
+  :
+    pf_consistent_strong2 th.
+Proof.
+  ii. exploit Memory.max_full_timemap_exists; eauto. intros MAX. des.
+  ii. exploit Memory.max_full_timemap_exists.
+  { eapply le_inhabited; eauto. eapply Memory.cap_le; eauto. refl. }
+  i. des. exploit CONSISTENT; eauto. i.
+  destruct x as [e2 [STEPS GOOD]]. guardH GOOD. des.
+  eapply pf_step_promise_free_step_rtc in STEPS.
+  eapply pf_steps_cancels_not_cancels in STEPS. des.
+  assert (NORESERVE: no_reserves th1.(Thread.memory)).
+  { ii. clarify. exploit steps_not_cancel_reserves_same; eauto.
+    i. des. clarify.
+
+
+  destruct th1. ss.
+  eapply hold_or_not with (Q := no_acq_read_msgs (caps_loc (Thread.memory th) (Local.promises (Thread.local th))) /1\ no_sc) in STEPS2. des.
+
+  - destruct e2. ss.
+    eapply pred_step_rtc_mon with (Q:=(promise_free /1\ (fun e => ~ is_cancel e) /1\ no_acq_read_msgs (caps_loc memory (Local.promises local))) /1\ no_sc) in HOLD; cycle 1.
+    { i. des. esplits; eauto. }
+    exploit no_sc_any_sc_rtc; try eapply HOLD; eauto. i. des.
+    esplits; eauto. unguard. des.
+    + left. ss. inv FAILURE; inv STEP0. inv LOCAL. eauto.
+    + right. esplits; eauto.
+
+  - exploit Thread.rtc_tau_step_future.
+    { eapply thread_steps_pred_steps. eapply STEPS0. }
+    { ss. eapply Local.cap_wf; eauto. }
+    { ss. eapply Memory.max_full_timemap_closed; eauto. }
+    { ss. eapply Memory.cap_closed; eauto. }
+    i. des. ss. inv STEP.
+    exploit Thread.step_future; eauto.
+    i. des.
+
+    hexploit (@rtc_tau_step_promise_consistent _ e3 e2); eauto.
+    { eapply thread_steps_pred_steps; eauto. }
+    { unguard. des.
+      - inv FAILURE; inv STEP. inv LOCAL. inv LOCAL0. ss.
+      - ii. rewrite PROMISES in *.
+        erewrite Memory.bot_get in PROMISE. clarify. } intros PROMS.
+
+    assert (RESERVES: only_reserves e2'.(Thread.local).(Local.promises)).
+    { econs.
+      - i. destruct msg; auto. exfalso. dup STEPS0.
+        eapply pf_step_rtc_promises_decrease in STEPS0; cycle 1.
+        { econs; eauto. }
+        ss. inv STEPS0.
+        unfold no_sc, no_acq_read_msgs in BREAKQ. des_ifs; try by (exfalso; eauto).
+        + apply not_and_or in BREAKQ. des; clarify.
+          apply imply_to_and in BREAKQ. des. apply NNPP in BREAKQ0.
+          unfold caps_loc in *. des. dup CAPS.
+          eapply caps_unchangable in CAPS; eauto; cycle 1.
+          { inv WF. eauto. }
+          eapply unchangable_rtc_increase in STEPS2; eauto. inv STEPS2.
+          inv STEP0; inv STEP. ss. inv LOCAL.
+          inv LOCAL0. clarify. eapply caps_max_view in CAPS0; eauto; cycle 1.
+          { inv WF. eauto. } des.
+          clarify. eapply PROMS in GET. ss. des_ifs. ss.
+          exploit max_full_timemap_get.
+          * apply MAX.
+          * inv WF. eapply PROMISES. eauto.
+          * i. eapply Time.lt_strorder. eapply TimeFacts.lt_le_lt; eauto.
+            etrans; eauto. eapply TimeMap.join_r.
+        + apply not_and_or in BREAKQ. des; clarify.
+          apply imply_to_and in BREAKQ. des. apply NNPP in BREAKQ0.
+          unfold caps_loc in *. des. dup CAPS.
+          eapply caps_unchangable in CAPS; eauto; cycle 1.
+          { inv WF. eauto. }
+          eapply unchangable_rtc_increase in STEPS2; eauto. inv STEPS2.
+          inv STEP0; inv STEP. ss. inv LOCAL.
+          eapply write_step_promise_consistent in LOCAL2; eauto.
+          inv LOCAL1. clarify. eapply caps_max_view in CAPS0; eauto; cycle 1.
+          { inv WF. eauto. } des.
+          clarify. eapply LOCAL2 in GET. ss. des_ifs. ss.
+          exploit max_full_timemap_get.
+          * apply MAX.
+          * inv WF. eapply PROMISES. eauto.
+          * i. eapply Time.lt_strorder. eapply TimeFacts.lt_le_lt; eauto.
+            etrans; eauto. eapply TimeMap.join_r.
+        + apply not_and_or in BREAKQ. des; clarify. apply NNPP in BREAKQ.
+          inv STEP0; inv STEP. ss. inv LOCAL. inv LOCAL0. ss.
+          eapply PROMS in GET. ss. des_ifs. ss.
+          hexploit max_full_timemap_get; eauto.
+          * inv WF. eapply Memory.cap_le; eauto.
+          * i. eapply Time.lt_strorder. eapply TimeFacts.lt_le_lt; eauto.
+        + inv STEP0; inv STEP. ss. inv LOCAL. inv LOCAL0. ss.
+          eapply PROMS in GET. ss. des_ifs. ss.
+          hexploit max_full_timemap_get; eauto.
+          * inv WF. eapply Memory.cap_le; eauto.
+          * i. eapply Time.lt_strorder. eapply TimeFacts.lt_le_lt; eauto.
+      - inv WF2. eauto. }
+
+    destruct e2'. destruct local. ss.
+    eapply pred_step_rtc_mon with (Q:=(promise_free /1\ no_acq_read_msgs (caps_loc (Thread.memory th) (Local.promises (Thread.local th)))) /1\ no_sc) in STEPS0; cycle 1.
+    { i. des. esplits; eauto. }
+    eapply no_sc_any_sc_rtc in STEPS0; ss. des.
+      exploit reserves_cancelable; eauto.
+      { inv WF2. eauto. }
+      i. des. esplits.
+      * etrans.
+        { eapply STEP. }
+        { eapply pred_step_rtc_mon; eauto.
+          unfold is_cancel. i. des_ifs. }
+      * ss. eauto.
+Qed.
+
+
+Lemma progressable_in_added_rtc
+      lang st lc sc0 sc1 m0 m1 tm
+      (CONSISTENT: Thread.consistent (Thread.mk lang st lc sc0 m0))
+      (FUTURE: Memory.future m0 m1)
+  :
+    exists m2 e2,
+      (<<ADDED: rtc (added_memory tm) m1 m2>>) /\
+      (<<STEPS: rtc (Thread.tau_step (lang:=lang))
+                    (Thread.mk _ st lc sc1 m1) e2>>) /\
+      (<<PROMISES: Local.promises (Thread.local e2) = Memory.bot>>).
+Proof.
+Admitted.
+
+Inductive diff_after_promises (prom mem0 mem1: Memory.t)
+          (caps: Loc.t -> Time.t -> Time.t -> Message.t -> Prop): Prop :=
+| diff_after_promises_intro
+    (MLE: Memory.le mem0 mem1)
+    (DIFF: forall loc to from msg
+                  (GET: Memory.get loc to mem1 = Some (from, msg))
+                  (NONE: Memory.get loc to mem0 = None),
+        (<<CAP: caps loc to from msg>>) /\
+        (exists from' to' val released,
+            (<<PROM: Memory.get loc to' prom = Some (from', Message.full val released)>>)) /\
+        (<<AFTER: forall from' to' val released
+                         (PROM: Memory.get loc to' prom = Some (from', Message.full val released)),
+            (<<TLE: Time.le to' from>>) >>))
+.
+
+(* Memory.future *)
+
+(* Memory.future_get1 *)
+
+(* Lemma diff_after_promises_step st lc mem0 mem1 caps sc sc' *)
+(*       (CONSISTENT: Local.promise_consistent (Local.mk vw prom)) *)
+
+(*       Thread.state *)
+
+
+
+
+(* rtc_tau_step_promise_consistent *)
+(*      : forall (lang : language) (th1 th2 : Thread.t lang), *)
+(*        rtc (Thread.tau_step (lang:=lang)) th1 th2 -> *)
+(*        Local.promise_consistent (Thread.local th2) -> *)
+(*        Local.wf (Thread.local th1) (Thread.memory th1) -> *)
+(*        Memory.closed_timemap (Thread.sc th1) (Thread.memory th1) -> *)
+(*        Memory.closed (Thread.memory th1) -> Local.promise_consistent (Thread.local th1) *)
+
+
+
+
+
+(* Definition caps (mem0 prom : Memory.t) (l : Loc.t) (t from : Time.t) (msg : Message.t) := *)
+(*   forall mem1 (CAP: Memory.cap prom mem0 mem1), *)
+(*     (<<GET0: Memory.get l t mem0 = None>>) /\ *)
+(*     (<<GET1: Memory.get l t mem1 = Some (from, msg)>>). *)
+
+
+
+
+(* pf_ *)
+
+(* Definition pf_consistent_strong lang (e:Thread.t lang): Prop := *)
+(*   forall mem1 sc1 *)
+(*          (CAP: Memory.cap e.(Thread.local).(Local.promises) e.(Thread.memory) mem1), *)
+(*   exists e2, *)
+(*     (<<STEPS: rtc (tau (@pred_step ((promise_free /1\ no_acq_read_msgs (caps_loc e.(Thread.memory) e.(Thread.local).(Local.promises))) /1\ no_sc) lang)) (Thread.mk _ e.(Thread.state) e.(Thread.local) sc1 mem1) e2>>) /\ *)
+(*     ((<<FAILURE: Local.failure_step e2.(Thread.local)>>) \/ *)
+(*      (<<PROMISES: e2.(Thread.local).(Local.promises) = Memory.bot>>)). *)
